SystemF/LocallyClosed.lean
@@ -33,6 +33,19 @@ inductive LcTm : Tm → Prop where
   | tApp t T : LcTm t → LcTy T → LcTm (t⦃T⦄)
   | tLam (L : Finset Name) t : (∀ X ∉ L, LcTm (t⟪$T X⟫)) → LcTm (Λ' t)
 
+/-
+  All bound *term* indices in `t` are strictly less than `k`.
+  Note: it ignores bound type variables, so `LcAtTm 0` is not equivalent to `LcTm` as
+  we would expect.
+-/
+inductive LcAtTm : ℕ → Tm → Prop where
+  | bvar i k : i < k → LcAtTm k (#v i)
+  | fvar x k : LcAtTm k ($v x)
+  | app t₁ t₂ k : LcAtTm k t₁ → LcAtTm k t₂ → LcAtTm k (t₁ ◦ t₂)
+  | lam T t k : LcAtTm (k + 1) t → LcAtTm k (ƛ T => t)
+  | tApp t T k : LcAtTm k t → LcAtTm k (t ⦃T⦄)
+  | tLam t k : LcAtTm k t → LcAtTm k (Λ' t)
+
 -- Example: `∀. 0 -> 0` is a locally closed type
 example : LcTy (∀' (#T 0 ⇒ #T 0)) := by
   apply LcTy.all ∅
@@ -86,7 +99,7 @@ theorem lcAtTy_openTy_id {T : Ty} {k : ℕ} (h : LcAtTy k T) (n : ℕ) (hn : k �
   If opening `T` yields a locally closed type at index `k`,
   then `T` is locally closed at index `k + 1`.
 -/
-theorem lcAtTy_of_open {T : Ty} {X : Name} {k : ℕ}
+theorem lcAtTy_of_openTy {T : Ty} {X : Name} {k : ℕ}
     (h : LcAtTy k (T⟪k, $TX⟫)) : LcAtTy (k + 1) T := by
   induction T generalizing k with
   | bvar _ =>
@@ -131,7 +144,7 @@ lemma lcAtTy_weaken {T : Ty} {k n : ℕ} (h : LcAtTy k T) (hle : k ≤ n) :
   If `T` is locally closed at index `k + 1` and `U` is locally closed,
   then opening `T` at index `k` with `U` yields a type that is locally closed at index `k`.
 -/
-lemma lcAtTy_open_inv_aux {k : ℕ} {T U : Ty}
+lemma lcAtTy_openTy_inv_aux {k : ℕ} {T U : Ty}
   (hT : LcAtTy (k + 1) T) (hU : LcAtTy 0 U) : LcAtTy k (T⟪k, U⟫) := by
   induction T generalizing k with
   | bvar idx =>
@@ -162,8 +175,8 @@ lemma lcAtTy_open_inv_aux {k : ℕ} {T U : Ty}
 /-
   If `T` has a bound variable, then opening `T` with a free variable yields a locally closed type.
 -/
-lemma lcAtTy_open_inv {T : Ty} {X : Name} (h : LcAtTy 1 T) : LcAtTy 0 (T⟪$T X⟫) := by
-  apply lcAtTy_open_inv_aux
+lemma lcAtTy_openTy_inv {T : Ty} {X : Name} (h : LcAtTy 1 T) : LcAtTy 0 (T⟪$T X⟫) := by
+  apply lcAtTy_openTy_inv_aux
   · assumption
   · constructor
 
@@ -179,7 +192,7 @@ theorem lcTy_implies_lcAtTy0 {T : Ty} (h : LcTy T) : LcAtTy 0 T := by
   | all L T _ ih =>
     apply LcAtTy.all
     have ⟨X, hX⟩ := exists_fresh_name L
-    apply lcAtTy_of_open
+    apply lcAtTy_of_openTy
     exact ih X hX
 
 /-
@@ -196,7 +209,7 @@ theorem lcAtTy0_implies_lcTy {T : Ty} (h : LcAtTy 0 T) : LcTy T := by
   | all T k h =>
     apply LcTy.all ∅
     intro X hX
-    have := lcAtTy_open_inv (X := X) h
+    have := lcAtTy_openTy_inv (X := X) h
     exact lcAtTy0_implies_lcTy this
 termination_by T.size
 decreasing_by
@@ -257,7 +270,7 @@ theorem openTy_substTy_comm {k} {X Y : Name} {T U : Ty} (hNeq : X ≠ Y) (hU : L
     rw [ih]
 
 /-
-  Substitution preserves locally closeness of types
+  Substitution preserves locally closedness of types
 -/
 theorem substTy_lcTy {T U : Ty} {X : Name} (hT : LcTy T) (hU : LcTy U) : LcTy (T[X ↦ U]) := by
   induction hT with
@@ -343,5 +356,161 @@ theorem openTy_lcTy {T U : Ty} (hT : LcTy (∀' T)) (hU : LcTy U) : LcTy (T⟪U�
     rw [←substTy_openTy_var (X := X) (by aesop)]
     apply this
 
+theorem lcAtTm_openTm_id {t : Tm} {k : ℕ} (h : LcAtTm k t) (n : ℕ) (hn : k ≤ n) (u : Tm) :
+    t⟪n, u⟫ = t := by
+  induction h generalizing n with
+  | bvar i k _ =>
+    simp only [openTm_bvar, beq_iff_eq, ite_eq_right_iff]
+    intro h
+    omega
+  | fvar x k => simp
+  | app t₁ t₂ k _ _ ih₁ ih₂ =>
+    simp only [openTm_app, Tm.app.injEq]
+    rw [ih₁ _ hn, ih₂ _ hn]
+    simp_all only [and_self]
+  | lam T t k _ ih =>
+    simp only [openTm_lam, Tm.lam.injEq, true_and]
+    rw [ih (n + 1) (by omega)]
+  | tApp t T k _ ih =>
+    simp only [openTm_tApp, Tm.tApp.injEq, and_true]
+    rw [ih _ hn]
+  | tLam t k _ ih =>
+    simp only [openTm_tLam, Tm.tLam.injEq]
+    rw [ih _ hn]
+
+theorem lcAtTm_of_openTm {t : Tm} {x : Name} {k : ℕ}
+    (h : LcAtTm k (t⟪k, $vx⟫)) : LcAtTm (k + 1) t := by
+  induction t generalizing k with
+  | bvar idx =>
+    simp only [openTm_bvar, beq_iff_eq] at h
+    split at h
+    · constructor
+      omega
+    · cases h
+      constructor
+      omega
+  | fvar name => constructor
+  | app t₁ t₂ t₁_ih t₂_ih =>
+    cases h
+    constructor
+    · apply t₁_ih
+      assumption
+    · apply t₂_ih
+      assumption
+  | tApp t T ih =>
+    cases h
+    constructor
+    · apply ih
+      assumption
+  | lam T t ih =>
+    cases h
+    constructor
+    apply ih
+    assumption
+  | tLam t ih =>
+    cases h
+    constructor
+    apply ih
+    assumption
+
+lemma lcAtTm_openTmTy_inv {t : Tm} {X : Name} {k n : ℕ}
+    (h : LcAtTm k (t⟪n, $TX⟫)) : LcAtTm k t := by
+  induction t generalizing k n with
+  | bvar idx =>
+    simp at h
+    assumption
+  | fvar name =>
+    simp at h
+    assumption
+  | app t₁ t₂ t₁_ih t₂_ih =>
+    cases h
+    constructor
+    · apply t₁_ih
+      assumption
+    · apply t₂_ih
+      assumption
+  | tApp t T ih =>
+    cases h
+    constructor
+    · apply ih
+      assumption
+  | lam T t ih =>
+    cases h
+    constructor
+    apply ih
+    assumption
+  | tLam t ih =>
+    cases h
+    constructor
+    apply ih
+    assumption
+
+theorem lcTm_implies_lcAtTm0 {t : Tm} (h : LcTm t) : LcAtTm 0 t := by
+  induction h with
+  | fvar x => constructor
+  | app t₁ t₂ _ _ ih₁ ih₂ =>
+    constructor
+    · apply ih₁
+    · apply ih₂
+  | lam L T t _ _ ih =>
+    have ⟨x, hx⟩ := exists_fresh_name L
+    specialize ih x hx
+    constructor
+    apply lcAtTm_of_openTm
+    exact ih
+  | tApp t T _ _ ih =>
+    constructor
+    assumption
+  | tLam L t _ ih =>
+    have ⟨X, hX⟩ := exists_fresh_name L
+    specialize ih X hX
+    constructor
+    apply lcAtTm_openTmTy_inv
+    exact ih
+
+/-
+  The converse does not hold: we don't track closedness of type variables in `LcAtTm`.
+-/
+theorem lcAtTm0_does_not_imply_lcTm : ∃ t, (LcAtTm 0 t ∧ ¬ LcTm t) := by
+  use ƛ (#T 0) => $v "x"
+  constructor
+  · constructor
+    constructor
+  · intro h
+    cases h with
+    | lam L T t h₁ h₂ =>
+      cases h₁
+
+@[simp]
+theorem openTm_lcTm_id {u : Tm} (h : LcTm u) (k : ℕ) (v : Tm) :
+    u⟪k, v⟫ = u := by
+  apply lcAtTm_openTm_id
+  · apply lcTm_implies_lcAtTm0 h
+  · simp only [zero_le]
+
+theorem openTm_substTm_comm {t u v : Tm} {X : Name} {k : ℕ} (hu : LcTm u) :
+    (t[X ↦ u])⟪k, v[X ↦ u]⟫ = (t⟪k, v⟫)[X ↦ u]:= by
+  induction t generalizing k with
+  | bvar idx =>
+    simp
+    split <;> rfl
+  | fvar name =>
+    simp only [substTm_fvar, beq_iff_eq, openTm_fvar]
+    split
+    · rw [openTm_lcTm_id hu]
+    · simp
+  | app t₁ t₂ t₁_ih t₂_ih =>
+    simp only [substTm_app, openTm_app, Tm.app.injEq]
+    rw [t₁_ih, t₂_ih]
+    simp_all only [and_self]
+  | tApp t T ih =>
+    simp only [substTm_tApp, openTm_tApp, Tm.tApp.injEq, and_true]
+    rw [ih]
+  | lam T t ih =>
+    simp only [substTm_lam, openTm_lam, Tm.lam.injEq, true_and]
+    rw [ih]
+  | tLam t ih =>
+    simp only [substTm_tLam, openTm_tLam, Tm.tLam.injEq]
+    rw [ih]
 
 end SystemF
